Removed lots of useless code and lemmas about splay trees or moved it somewhere else. Added a TODO file. Refactored a few things about BSTs (particularly removed BTree_toList - use inorder instead). Renamed BinomialTree into BinomialHeap2.

DS/BST/SplayTree.v
@@ -8,7 +8,7 @@ Set Implicit Arguments.
 
 Definition SplayTree (A : Type) : Type := BTree A.
 
-Function partition {A : Type} (p : A -> A -> bool) (pivot : A) (h : SplayTree A)
+Function splay {A : Type} (p : A -> A -> bool) (pivot : A) (h : SplayTree A)
   : SplayTree A * SplayTree A :=
 match h with
     | empty => (empty, empty)
@@ -20,10 +20,10 @@ match h with
               | node y b1 b2 =>
                   if p y pivot
                   then
-                    let '(small, big) := partition p pivot b2
+                    let '(small, big) := splay p pivot b2
                     in (node y (node x a b1) small, big)
                   else
-                    let '(small, big) := partition p pivot b1
+                    let '(small, big) := splay p pivot b1
                     in (node x a small, node y big b2)
           end
         else
@@ -32,214 +32,101 @@ match h with
               | node y a1 a2 =>
                   if p y pivot
                   then
-                    let '(small, big) := partition p pivot a2
+                    let '(small, big) := splay p pivot a2
                     in (node y a1 small, node x big b)
                   else
-                    let '(small, big) := partition p pivot a1
+                    let '(small, big) := splay p pivot a1
                     in (small, node y big (node x a2 b))
           end
-end.
-
-Definition isEmpty
-  {A : Type} (h : SplayTree A) : bool :=
-match h with
-    | empty => true
-    | _ => false
 end.
 
 Definition insert
   {A : Type} (p : A -> A -> bool) (x : A) (h : SplayTree A) : SplayTree A :=
     let
-      (smaller, bigger) := partition p x h
+      (smaller, bigger) := splay p x h
     in
       node x smaller bigger.
-
-Function findMin'
-  {A : Type} (h : SplayTree A) : option A :=
-match h with
-    | empty => None
-    | node m empty _ => Some m
-    | node _ l _ => findMin' l
-end.
-
-Function findMin
-  {A : Type} (h : SplayTree A) : option A :=
-match h with
-    | empty => None
-    | node v l r =>
-        match findMin l with
-            | None => Some v
-            | Some m => Some m
-        end
-end.
-
-Function deleteMin
-  {A : Type} (h : SplayTree A) : SplayTree A :=
-match h with
-    | empty => empty
-    | node _ empty r => r
-    | node v l r => node v (deleteMin l) r
-end.
-
-Function deleteMin'
-  {A : Type} (h : SplayTree A) : option A * SplayTree A :=
-match h with
-    | empty => (None, empty)
-    | node m empty r => (Some m, r)
-    | node v l r =>
-        let '(min, l') := deleteMin' l in (min, node v l' r)
-end.
-
-Function deleteMin2
-  {A : Type} (h : SplayTree A) : option (A * SplayTree A) :=
-match h with
-    | empty => None
-    | node v l r =>
-        match deleteMin2 l with
-            | None => Some (v, r)
-            | Some (min, l') => Some (min, node v l' r)
-        end
-end.
 
 Function merge {A : Type} (p : A -> A -> bool) (h1 h2 : SplayTree A) : SplayTree A :=
 match h1 with
     | empty => h2
     | node v l r =>
         let
-          (l', r') := partition p v h2
+          (l', r') := splay p v h2
         in
           node v (merge p l l') (merge p r r')
 end.
 
 (** Properties of [isEmpty] *)
 
-Lemma isEmpty_partition_true :
-  forall (A : Type) (p : A -> A -> bool) (x : A) (h l r : SplayTree A),
-    partition p x h = (l, r) ->
-      isEmpty h = true <-> isEmpty l = true /\ isEmpty r = true.
+Lemma isEmpty_splay :
+  forall {A : Type} {cmp : A -> A -> comparison} {x : A} {h l r : SplayTree A},
+    splay cmp x h = (l, r) ->
+      isEmpty h = isEmpty l && isEmpty r.
 Proof.
-  split; intros; functional induction @partition A p x h; inv H; firstorder.
-    all: cbn in *; congruence.
-Qed.
-
-Lemma isEmpty_partition_false :
-  forall (A : Type) (p : A -> A -> bool) (x : A) (h l r : SplayTree A),
-    partition p x h = (l, r) ->
-      isEmpty h = false <-> isEmpty l = false \/ isEmpty r = false.
-Proof.
-  split; intros; functional induction @partition A p x h; inv H; firstorder.
+  intros until h.
+  functional induction splay cmp x h;
+  inv 1. cbn.
+    rewrite andb_false_r. reflexivity.
 Qed.
 
 Lemma isEmpty_insert :
   forall (A : Type) (p : A -> A -> bool) (x : A) (h : SplayTree A),
     isEmpty (insert p x h) = false.
 Proof.
-  intros. unfold insert. case_eq (partition p x h); intros small big H.
+  intros. unfold insert. case_eq (splay p x h); intros small big H.
   cbn. reflexivity.
 Qed.
 
-Lemma isEmpty_merge_true :
-  forall (A : Type) (p : A -> A -> bool) (h1 h2 : SplayTree A),
-    isEmpty (merge p h1 h2) = true <->
-      isEmpty h1 = true /\ isEmpty h2 = true.
+Lemma isEmpty_merge :
+  forall {A : Type} {cmp : A -> A -> bool} {h1 h2 : SplayTree A},
+    isEmpty (merge cmp h1 h2) = isEmpty h1 && isEmpty h2.
 Proof.
-  destruct h1; cbn; intros; try destruct (partition p a h2); firstorder.
-    cbn in H. congruence.
+  destruct h1; cbn.
+    reflexivity.
+    intro. destruct (splay _ _ _). cbn. reflexivity.
 Qed.
 
-Lemma isEmpty_merge_false :
-  forall (A : Type) (p : A -> A -> bool) (h1 h2 : SplayTree A),
-    isEmpty (merge p h1 h2) = false <->
-      isEmpty h1 = false \/ isEmpty h2 = false.
-Proof.
-  destruct h1; cbn; intros; try destruct (partition p a h2); firstorder congruence. 
-Qed.
+(** Properties of [splay]. *)
 
-Lemma isEmpty_size :
-  forall (A : Type) (h : SplayTree A),
-    isEmpty h = true <-> size h = 0.
-Proof.
-  split; destruct h; cbn in *; intros; congruence.
-Qed.
-
-Lemma isEmpty_countBT :
-  forall (A : Type) (p : A -> bool) (t : SplayTree A),
-    isEmpty t = true -> countBT p t = 0.
-Proof.
-  destruct t; trich.
-Qed.
-
-(** Properties of [partition]. *)
-
-Lemma Elem_partition :
+Lemma Elem_splay :
   forall (A : Type) (p : A -> A -> bool) (x pivot : A) (h l r : SplayTree A),
-    partition p pivot h = (l, r) ->
+    splay p pivot h = (l, r) ->
       Elem x h <-> Elem x l \/ Elem x r.
 Proof.
   split; revert x l r H.
-    functional induction @partition A p pivot h; inv 1;
+    functional induction @splay A p pivot h; inv 1;
       rewrite e3 in *; inv 1; inv H1; edestruct IHp0; eauto.
-    functional induction @partition A p pivot h; inv 1; inv 1;
+    functional induction @splay A p pivot h; inv 1; inv 1;
       rewrite ?e3 in *; inv H0; eauto 6; inv H1.
 Qed.
 
-Ltac aux := intros; repeat
-match goal with
-    | H : context [?x ≤? ?y] |- _ => trich
-(*         let H' := fresh "H" in
-          destruct (leqb_spec x y) as [H' | H']; try congruence;
-          clear H; rename H' into H
- *)    | H : ~ _ ≤ _ |- _ => trich (* apply Ord_not_leq_lt in H *)
-    | H : elem _ ?t, H' : forall _, elem _ ?t -> _ |- _ =>
-        specialize (H' _ H)
-    | H : ?a ≤ ?b, H' : ?b ≤ ?c |- ?a ≤ ?c => trich
-(*         apply leq_trans with b; assumption *)
-    | H : elem _ empty |- _ => inv H
-    | H : elem _ (node _ _ _) |- _ => inv H
-    | H : isBST ?x, H' : isBST ?x -> _ |- _ => specialize (H' H)
-    | H : isBST empty |- _ => inv H
-    | H : isBST (node _ _ _) |- _ => inv H
-end; auto.
-
-Lemma isBST_partition :
-  forall (A : Type) (p : A -> A -> comparison) (x : A) (h l r : SplayTree A),
-    partition p x h = (l, r) -> isBST p h -> isBST p (node x l r).
+Lemma isBST_splay :
+  forall {A : Type} {cmp : A -> A -> comparison} {x : A} {h l r : SplayTree A},
+    splay cmp x h = (l, r) ->
+      isBST cmp h -> isBST cmp (node x l r).
 Proof.
   intros until h.
-  functional induction partition p x h;
-  inv 1; isBST.
-    isBST'; Elems''. trich.
-(*   inv 1; inv 1; aux. constructor; auto.
-  try specialize (IHp0 _ _ _ e3 H7); try specialize (IHp0 _ _ _ e3 H9);
-  try inv IHp0; repeat constructor; aux. inv H.
- *)Admitted.
+  functional induction splay cmp x h;
+  inv 1.
+Admitted.
 
-Lemma size_partition :
+Lemma size_splay :
   forall (A : Type) (p : A -> A -> bool) (x : A) (h h1 h2 : SplayTree A),
-    partition p x h = (h1, h2) -> size h = size h1 + size h2.
+    splay p x h = (h1, h2) -> size h = size h1 + size h2.
 Proof.
   intros A p x h.
-  functional induction partition p x h; inv 1; cbn;
+  functional induction splay p x h; inv 1; cbn;
   erewrite IHp0; eauto; lia.
 Qed.
 
-Lemma countBT_partition :
-  forall (A : Type) (cmp : A -> A -> bool) (p : A -> bool) (pivot : A) (h h1 h2 : SplayTree A),
-    partition cmp pivot h = (h1, h2) ->
-      countBT p h = countBT p h1 + countBT p h2.
-Proof.
-  intros until h. revert p.
-  functional induction partition cmp pivot h;
-  inv 1; cbn; erewrite IHp; eauto;
-  destruct (p x), (p y); cbn; unfold id; lia.
-Qed.
-
 (** Properties of [insert]. *)
+
 Lemma Elem_insert :
   forall (A : Type) (p : A -> A -> bool) (x : A) (h : SplayTree A),
     Elem x (insert p x h).
 Proof.
-  intros. unfold insert. destruct (partition p x h). constructor.
+  intros. unfold insert. destruct (splay p x h). constructor.
 Qed.
 
 Lemma isBST_insert :
@@ -247,8 +134,8 @@ Lemma isBST_insert :
     isBST p h -> isBST p (insert p x h).
 Proof.
   intros. unfold insert.
-  destruct (partition p x h) eqn: Heq.
-  eapply isBST_partition; eauto.
+  destruct (splay p x h) eqn: Heq.
+  eapply isBST_splay; eauto.
 Qed.
 
 Lemma size_insert :
@@ -256,20 +143,9 @@ Lemma size_insert :
     size (insert p x h) = 1 + size h.
 Proof.
   intros. unfold insert.
-  destruct (partition p x h) as [smaller bigger] eqn: Heq.
+  destruct (splay p x h) as [smaller bigger] eqn: Heq.
   cbn. f_equal. symmetry.
-  eapply size_partition. eassumption.
-Qed.
-
-Lemma countBT_insert :
-  forall (A : Type) (cmp : A -> A -> bool) (p : A -> bool) (x : A) (h : SplayTree A),
-    countBT p (insert cmp x h) =
-    (if p x then 1 else 0) + countBT p h.
-Proof.
-  intros. unfold insert.
-  destruct (partition cmp x h) eqn: Heq.
-  apply (countBT_partition cmp p) in Heq.
-  rewrite Heq. cbn. destruct (p x); reflexivity.
+  eapply size_splay. eassumption.
 Qed.
 
 (** Properties of [merge]. *)
@@ -280,12 +156,12 @@ Lemma Elem_merge :
 Proof.
   split; revert x.
     functional induction merge p h1 h2; inv 1.
-      edestruct IHs; eauto. right. eapply Elem_partition; eauto.
-      edestruct IHs0; eauto. right. eapply Elem_partition; eauto.
+      edestruct IHs; eauto. right. eapply Elem_splay; eauto.
+      edestruct IHs0; eauto. right. eapply Elem_splay; eauto.
     functional induction merge p h1 h2; inv 1.
       inv H0.
       inv H0.
-      erewrite (Elem_partition _ _ _ _ e0) in H0. inv H0.
+      erewrite (Elem_splay _ _ _ _ e0) in H0. inv H0.
 Qed.
 
 Lemma isBST_merge :
@@ -295,12 +171,12 @@ Proof.
   intros until h2.
   functional induction merge p h1 h2; inv 1; intro.
   constructor.
-    apply IHs; eauto. eapply isBST_partition in e0; inv e0.
+    apply IHs; eauto. eapply isBST_splay in e0; inv e0.
     intros. apply Elem_merge in H0. inv H0.
-      apply isBST_partition in e0; auto. inv e0.
-    apply IHs0; eauto. eapply isBST_partition in e0; inv e0.
+      apply isBST_splay in e0; auto. inv e0.
+    apply IHs0; eauto. eapply isBST_splay in e0; inv e0.
     intros. apply Elem_merge in H0. inv H0.
-      apply isBST_partition in e0; auto. inv e0.
+      apply isBST_splay in e0; auto. inv e0.
 Qed.
 
 Lemma size_merge :
@@ -309,213 +185,5 @@ Lemma size_merge :
 Proof.
   intros. functional induction merge p h1 h2; cbn.
     reflexivity.
-    apply size_partition in e0. lia.
+    apply size_splay in e0. lia.
 Qed.
-
-Lemma countBT_merge :
-  forall (A : Type) (cmp : A -> A -> bool) (p : A -> bool) (h1 h2 : SplayTree A),
-    countBT p (merge cmp h1 h2) = countBT p h1 + countBT p h2.
-Proof.
-  intros until h2.
-  functional induction (merge cmp h1 h2); cbn.
-    reflexivity.
-    apply (countBT_partition cmp p) in e0.
-      destruct (p v); unfold id; lia.
-Qed.
-
-(** Properties of [findMin] *)
-
-Lemma Elem_findMin :
-  forall (A : Type) (m : A) (h : SplayTree A),
-    findMin h = Some m -> Elem m h.
-Proof.
-  intros. functional induction @findMin A h; inv H.
-Qed.
-
-Lemma Elem_findMin_node :
-  forall (A : Type) (m v : A) (l r : SplayTree A),
-    findMin (node v l r) = Some m -> m = v \/ Elem m l.
-Proof.
-  intros. remember (node v l r) as h. revert m v l r Heqh H.
-  functional induction (findMin h); inv 1; inv 1.
-  functional inversion e0; subst; eauto.
-  edestruct IHo; eauto. subst. eauto.
-Qed.
-
-Lemma findMin_aux :
-  forall (A : Type) (v : A) (l r : SplayTree A),
-    findMin (node v l r) = Some v \/
-    findMin (node v l r) = findMin l.
-Proof.
-  intros. remember (node v l r) as h.
-  functional induction @findMin A h; inv Heqh.
-Qed.
-
-Lemma findMin_spec :
-  forall {A : Ord} {h : SplayTree A} {m : A},
-    findMin h = Some m ->
-      isBST cmp h -> forall x : A, Elem x h -> cmp m x <> Gt.
-Proof.
-  intros A h.
-  functional induction findMin h; inv 1; inv 1.
-    inv 1.
-      trich.
-      functional inversion e0. subst. inv H1.
-      specialize (H6 _ H1). intro. trich.
-    inv 1.
-      apply Elem_findMin in e0. rewrite (H4 _ e0). inv 1.
-      apply Elem_findMin in e0. specialize (H4 _ e0). specialize (H6 _ H1).
-        trich.
-Qed.
-
-(** Properties of [findMin']. *)
-
-Lemma findMin'_elem :
-  forall (A : Type) (m : A) (h : SplayTree A),
-    findMin' h = Some m -> Elem m h.
-Proof.
-  intros. functional induction @findMin' A h; inv H.
-Qed.
-
-Lemma findMin'_elem_node :
-  forall (A : Type) (m v : A) (l r : SplayTree A),
-    findMin' (node v l r) = Some m -> m = v \/ Elem m l.
-Proof.
-  intros. remember (node v l r) as h. revert m v l r Heqh H.
-  functional induction @findMin' A h; inv 1; intros.
-    inv H.
-    inv H. destruct l0; cbn in *.
-      congruence.
-        destruct (IHo _ _ _ _ eq_refl H1); subst; auto.
-Qed.
-
-Lemma findMin'_aux :
-  forall (A : Type) (v : A) (l r : SplayTree A),
-    findMin' (node v l r) = Some v \/
-    findMin' (node v l r) = findMin' l.
-Proof.
-  intros. remember (node v l r) as h.
-  functional induction @findMin' A h; inv Heqh.
-Qed.
-
-Lemma findMin'_spec :
-  forall (A : Type) (cmp : A -> A -> comparison) (m : A) (h : SplayTree A),
-    isBST cmp h -> findMin' h = Some m ->
-      forall x : A, Elem x h -> cmp m x.
-Proof.
-  intros A cmp m h. revert m.
-  functional induction findMin' h; inv 1; inv 1.
-    inv 1.
-      admit.
-      inv H1.
-      admit.
-    specialize (H4 _ (findMin'_elem _ H1)). inv 1.
-      red. rewrite H4. cbn. reflexivity.
-      specialize (H6 _ H2). admit. (* transitivity *)
-Admitted.
-
-(** Properties of [deleteMin2]. *)
-
-Lemma deleteMin2_size :
-  forall (A : Type) (m : A) (h h' : SplayTree A),
-    deleteMin2 h = Some (m, h') -> size h = 1 + size h'.
-Proof.
-  intros A m h. revert m.
-  functional induction @deleteMin2 A h; cbn; inv 1.
-    destruct l; cbn in *.
-      reflexivity.
-      destruct (deleteMin2 l1).
-        destruct p. congruence.
-        congruence.
-    rewrite (IHo _ _ e0). cbn. reflexivity.
-Qed.
-
-Lemma deleteMin2_isEmpty_None :
-  forall (A : Type) (h : SplayTree A),
-    deleteMin2 h = None -> isEmpty h = true.
-Proof.
-  intros. functional induction @deleteMin2 A h; cbn; inv H.
-Qed.
-
-Lemma deleteMin2_isEmpty_Some :
-  forall (A : Type) (m : A) (h h' : SplayTree A),
-    deleteMin2 h = Some (m, h') -> isEmpty h = false.
-Proof.
-  intros. functional induction @deleteMin2 A h; cbn; inv H.
-Qed.
-
-Lemma deleteMin2_elem :
-  forall (A : Type) (m : A) (h h' : SplayTree A),
-    deleteMin2 h = Some (m, h') -> Elem m h.
-Proof.
-  intros A m h. revert m.
-  functional induction @deleteMin2 A h; inv 1; eauto.
-Qed.
-
-Lemma deleteMin2_elem_node :
-  forall (A : Type) (m v : A) (l r h' : SplayTree A),
-    deleteMin2 (node v l r) = Some (m, h') -> m = v \/ Elem m l.
-Proof.
-  intros. remember (node v l r) as h. revert m v l r h' Heqh H.
-  functional induction @deleteMin2 A h; inv 1; intros.
-    inv H.
-    inv H. destruct l0; cbn in *.
-      congruence.
-      destruct (deleteMin2 l0_1); inv e0. destruct p. inv H0.
-        destruct (IHo _ _ _ _ _ eq_refl eq_refl); subst; auto.
-Qed.
-
-Lemma deleteMin2_aux :
-  forall (A : Type) (v : A) (l r : SplayTree A),
-    deleteMin2 (node v l r) = Some (v, r) \/
-    deleteMin2 (node v l r) =
-      match deleteMin2 l with
-          | None => Some (v, r)
-          | Some (m, l') => Some (m, node v l' r)
-      end.
-Proof.
-  intros. remember (node v l r) as h. revert v l r Heqh.
-  functional induction @deleteMin2 A h; inv 1.
-  destruct l0; cbn in *.
-    congruence.
-    specialize (IHo _ _ _ eq_refl). destruct (deleteMin2 l0_1).
-      destruct p. inv e0.
-      inv e0.
-Qed.
-
-Lemma deleteMin2_spec :
-  forall (A : Type) (cmp : A -> A -> comparison) (m : A) (h h' : SplayTree A),
-    isBST cmp h -> deleteMin2 h = Some (m, h') ->
-      forall x : A, Elem x h -> cmp m x.
-Proof.
-  intros A cmp m h. revert m.
-  functional induction deleteMin2 h; inv 1; intros.
-    inv H. inv H0.
-      admit.
-      functional inversion e0; subst. inv H1.
-      specialize (H6 _ H1). admit. (* flip H6 *)
-      inv H. inv H0.
-        rewrite H4. reflexivity. eapply deleteMin2_elem. eassumption.
-        eapply IHo; eauto.
-        specialize (H6 _ H1). apply deleteMin2_elem in e0. specialize (H4 _ e0). admit. (* transitivity *)
-Admitted.
-
-Lemma deleteMin2_countBT :
-  forall (A : Type) (cmp : A -> A -> comparison) (p : A -> bool) (m : A) (h h' : SplayTree A),
-    isBST cmp h -> deleteMin2 h = Some (m, h') ->
-      countBT p h =
-      (if p m then 1 else 0) + countBT p h'.
-Proof.
-(* TODO
-  intros A p m h. revert p m.
-  functional induction deleteMin2 h; cbn; inv 1; intros.
-    destruct l; cbn in *.
-      inv H. destruct (p m); reflexivity.
-      destruct (deleteMin2 l1). try destruct p; inv e0.
-    inv H. destruct l; cbn in *.
-      inv e0.
-      destruct (deleteMin2 l1); try destruct p;
-      inv e0; specialize (IHo x _ _ ltac:(inv H4) eq_refl);
-      rewrite IHo; trich.
-*)
-Admitted.
