DS/BST/SplayTree2.v
@@ -7,27 +7,6 @@ Set Implicit Arguments.
 
 Definition SplayTree (A : Ord) : Type := BTree A.
 
-Function bigger
-  {A : Ord} (pivot : A) (h : SplayTree A) : SplayTree A :=
-match h with
-    | empty => empty
-    | node v l r =>
-        if v ≤? pivot
-        then bigger pivot r
-        else
-          match l with
-              | empty => node v empty r
-              | node v' l' r' =>
-                  if v' ≤? pivot
-                  then (* v' <= pivot < v *)
-                    node v (bigger pivot r') r
-                  else (* pivot < v' <= v *)
-                    node v' (bigger pivot l') (node v r' r)
-          end
-end.
-
-(* Compute bigger 2 (node 5 (node 2 empty empty) empty). *)
-
 Function smaller
   {A : Ord} (pivot : A) (h : SplayTree A) : SplayTree A :=
 match h with
@@ -47,47 +26,191 @@ match h with
         else smaller pivot l
 end.
 
-Definition partition
+Function bigger
+  {A : Ord} (pivot : A) (h : SplayTree A) : SplayTree A :=
+match h with
+    | empty => empty
+    | node v l r =>
+        if v ≤? pivot
+        then bigger pivot r
+        else
+          match l with
+              | empty => node v empty r
+              | node v' l' r' =>
+                  if v' ≤? pivot
+                  then (* v' <= pivot < v *)
+                    node v (bigger pivot r') r
+                  else (* pivot < v' <= v *)
+                    node v' (bigger pivot l') (node v r' r)
+          end
+end.
+
+Definition splay
   {A : Ord} (x : A) (h : SplayTree A) : SplayTree A * SplayTree A:=
     (smaller x h, bigger x h).
 
 Definition insert
   {A : Ord} (x : A) (h : SplayTree A) : SplayTree A :=
-    let (smaller, bigger) := partition x h
+    let (smaller, bigger) := splay x h
     in node x smaller bigger.
-
-Function findMin
-  {A : Ord} (h : SplayTree A) : option A :=
-match h with
-    | empty => None
-    | node m empty _ => Some m
-    | node _ l _ => findMin l
-end.
-
-Function deleteMin
-  {A : Ord} (h : SplayTree A) : SplayTree A :=
-match h with
-    | empty => empty
-    | node _ empty r => r
-    | node v l r => node v (deleteMin l) r
-end.
-
-Function deleteMin'
-  {A : Ord} (h : SplayTree A) : option A * SplayTree A :=
-match h with
-    | empty => (None, empty)
-    | node m empty r => (Some m, r)
-    | node v l r =>
-        let '(min, l') := deleteMin' l in (min, node v l' r)
-end.
 
 Function merge {A : Ord} (h1 h2 : SplayTree A) : SplayTree A :=
 match h1 with
     | empty => h2
     | node v l r =>
-        let '(l', r') := partition v h2
+        let '(l', r') := splay v h2
         in node v (merge l l') (merge r r')
 end.
+
+(** Properties [bigger]. *)
+
+Lemma Elem_bigger :
+  forall {A : Ord} {pivot : A} {h : SplayTree A},
+    isBST cmp h ->
+      forall x : A,
+        Elem x (bigger pivot h)
+          <->
+        Elem x h /\ x > pivot.
+Proof.
+  intros until h.
+  functional induction bigger pivot h;
+  isBST; intro;
+  rewrite ?Elem_node, ?IHs; auto;
+  split; Elems'.
+Qed.
+
+Lemma isBST_bigger :
+  forall (A : Ord) (pivot : A) (h : SplayTree A),
+    isBST cmp h -> isBST cmp (bigger pivot h).
+Proof.
+  intros until h.
+  functional induction bigger pivot h;
+  isBST'; auto; intros.
+    apply Elem_bigger in H; firstorder.
+    apply Elem_bigger in H; firstorder.
+    inv H.
+      trich.
+      specialize (H6 _ H1). specialize (H4 v' ltac:(auto)). trich.
+Qed.
+
+(** Properties of [smaller]. *)
+
+Lemma Elem_smaller : (* TODO: fix definition of isBST *)
+  forall {A : Ord} {pivot : A} {h : SplayTree A},
+    isBST cmp h ->
+      forall x : A,
+        Elem x (smaller pivot h)
+          <->
+        Elem x h /\ x < pivot.
+Proof.
+  intros until h.
+  functional induction smaller pivot h;
+  isBST; intro;
+  rewrite ?Elem_node, ?IHs; auto;
+  split; Elems'.
+Admitted.
+
+Lemma isBST_smaller :
+  forall {A : Ord} {pivot : A} {h : SplayTree A},
+    isBST cmp h -> isBST cmp (smaller pivot h).
+Proof.
+  intros until h.
+  functional induction smaller pivot h;
+  isBST'; try intro;
+  rewrite ?Elem_smaller; Elems'.
+    specialize (H6 v' ltac:(auto)). trich.
+    specialize (H6 v' ltac:(auto)). trich.
+Qed.
+
+(** Properties of [splay]. *)
+
+Lemma Elem_splay :
+  forall {A : Ord} {pivot : A} {h l r : SplayTree A},
+    splay pivot h = (l, r) ->
+      isBST cmp h ->
+        forall x : A, Elem x h <-> Elem x l \/ Elem x r.
+Proof.
+  unfold splay.
+  inv 1. intros.
+  rewrite Elem_smaller, Elem_bigger.
+    2-3: assumption.
+    firstorder. destruct (cmp_spec x pivot).
+      admit. (* TODO: fix definition of isBST *)
+      left. split; try left; auto.
+      right; split; auto.
+Admitted.
+
+Lemma isBST_splay :
+  forall {A : Ord} {pivot : A} {h l r : SplayTree A},
+    splay pivot h = (l, r) ->
+      isBST cmp h -> isBST cmp (node pivot l r).
+Proof.
+  unfold splay.
+  inv 1. isBST'.
+    apply isBST_smaller. assumption.
+    intro. rewrite Elem_smaller; Elems'.
+    apply isBST_bigger. assumption.
+    intro. rewrite Elem_bigger; Elems'.
+Qed.
+
+(** Properties of [insert]. *)
+
+Lemma Elem_insert :
+  forall {A : Ord} {x : A} {h : SplayTree A},
+    isBST cmp h ->
+      forall y : A, Elem y (insert x h) <-> y = x \/ Elem y h.
+Proof.
+  unfold insert, splay. intros.
+  rewrite Elem_node, Elem_smaller, Elem_bigger; auto. split.
+    firstorder.
+    destruct (cmp_spec y x); firstorder.
+Qed.
+
+Lemma isBST_insert :
+  forall {A : Ord} {x : A} {h : SplayTree A},
+    isBST cmp h -> isBST cmp (insert x h).
+Proof.
+  intros.
+  unfold insert.
+  destruct (splay x h) eqn: Heq.
+  eapply isBST_splay; eassumption.
+Qed.
+
+(** Properties of [merge]. *)
+
+Lemma Elem_merge :
+  forall {A : Ord} {h1 h2 : SplayTree A} {x : A},
+    isBST cmp h1 -> isBST cmp h2 ->
+      Elem x (merge h1 h2)
+        <->
+      Elem x h1 \/ Elem x h2.
+Proof.
+  intros until h2.
+  functional induction merge h1 h2;
+  intro; isBST.
+    split; Elems.
+    {
+      pose (isBST_splay e0 H). inv i.
+      rewrite (Elem_splay e0 H), ?Elem_node, IHs, IHs0; auto.
+      split; Elems''.
+    }
+Qed.
+
+Lemma isBST_merge :
+  forall {A : Ord} {h1 h2 : SplayTree A},
+    isBST cmp h1 -> isBST cmp h2 ->
+      isBST cmp (merge h1 h2).
+Proof.
+  intros until h2.
+  functional induction merge h1 h2;
+  isBST.
+    assumption.
+    pose (isBST_splay e0 H). isBST'.
+      apply IHs; assumption.
+      intro. rewrite Elem_merge; Elems.
+      apply IHs0; assumption.
+      intro. rewrite Elem_merge; Elems.
+Qed.
 
 (** Properties of [isEmpty] *)
 
@@ -127,42 +250,13 @@ Proof.
   cbn in *; congruence.
 Qed.
 
-Lemma isEmpty_partition_true :
-  forall (A : Ord) (x : A) (h l r : SplayTree A),
-    partition x h = (l, r) ->
-      isEmpty h = true <-> isEmpty l = true /\ isEmpty r = true.
-Proof.
-  unfold partition. split; inv H; intros.
-    split.
-      apply isEmpty_smaller_true. assumption.
-      apply isEmpty_bigger_true. assumption.
-    destruct H.
-    induction h as [| v l IHl r IHr]; cbn in *.
-      reflexivity.
-      trich; [destruct r | destruct l]; trich.
-Qed.
-
-Lemma isEmpty_partition_false :
-  forall (A : Ord) (x : A) (h l r : SplayTree A),
-    partition x h = (l, r) ->
-      isEmpty h = false <-> isEmpty l = false \/ isEmpty r = false.
-Proof.
-  unfold partition. split; inv H; intros.
-    induction h as [| v l IHl r IHr]; cbn in *.
-      auto.
-      trich; [destruct r | destruct l]; trich.
-    destruct H.
-      eapply isEmpty_smaller_false. eassumption.
-      eapply isEmpty_bigger_false. eassumption.
-Qed.
-
-Lemma isEmpty_partition :
+Lemma isEmpty_splay :
   forall {A : Ord} {x : A} {h l r : SplayTree A},
-    partition x h = (l, r) ->
+    splay x h = (l, r) ->
       isEmpty h = isEmpty l && isEmpty r.
 Proof.
   intros until h.
-  unfold partition. inv 1.
+  unfold splay. inv 1.
   functional induction smaller x h;
   try destruct l; cbn; trich.
     destruct l2; cbn; trich.
@@ -173,26 +267,8 @@ Lemma isEmpty_insert :
   forall (A : Ord) (x : A) (h : SplayTree A),
     isEmpty (insert x h) = false.
 Proof.
-  intros. unfold insert. case_eq (partition x h); intros small big H.
+  intros. unfold insert. case_eq (splay x h); intros small big H.
   cbn. reflexivity.
-Qed.
-
-Lemma isEmpty_merge_true :
-  forall (A : Ord) (h1 h2 : SplayTree A),
-    isEmpty (merge h1 h2) = true <->
-      isEmpty h1 = true /\ isEmpty h2 = true.
-Proof.
-  destruct h1; cbn; intros; try destruct (partition c h2);
-  firstorder congruence.
-Qed.
-
-Lemma isEmpty_merge_false :
-  forall (A : Ord) (h1 h2 : SplayTree A),
-    isEmpty (merge h1 h2) = false <->
-      isEmpty h1 = false \/ isEmpty h2 = false.
-Proof.
-  destruct h1; cbn; intros; try destruct (partition c h2);
-  firstorder congruence.
 Qed.
 
 Lemma isEmpty_merge :
@@ -200,233 +276,4 @@ Lemma isEmpty_merge :
     isEmpty (merge h1 h2) = isEmpty h1 && isEmpty h2.
 Proof.
   destruct h1; cbn; reflexivity.
-Qed.
-
-Lemma isEmpty_size :
-  forall (A : Ord) (h : SplayTree A),
-    isEmpty h = true <-> size h = 0.
-Proof.
-  split; destruct h; cbn in *; intros; congruence.
-Qed.
-
-Lemma isEmpty_countBT :
-  forall (A : Ord) (p : A -> bool) (h : SplayTree A),
-    isEmpty h = true -> countBT p h = 0.
-Proof.
-  destruct h; cbn; congruence.
-Qed.
-
-(** Properties [bigger]. *)
-
-Lemma bigger_spec :
-  forall (A : Ord) (pivot : A) (h : SplayTree A),
-    isBST cmp h -> forall x : A, elem cmp x (bigger pivot h) ->
-      pivot < x.
-Proof.
-  intros until h.
-  functional induction bigger pivot h;
-  isBST; cbn; intros; trich.
-    specialize (IHs H8 _ H). trich.
-    specialize (IHs H2 _ H). trich.
-Qed.
-
-Lemma Elem_bigger' :
-  forall (A : Ord) (x pivot : A) (h : SplayTree A),
-    isBST cmp h -> Elem x (bigger pivot h) -> Elem x h.
-Proof.
-  intros until h.
-  functional induction bigger pivot h;
-  isBST; inv 1.
-    inv H1.
-Qed.
-
-Lemma Elem_bigger :
-  forall {A : Ord} {pivot : A} {h : SplayTree A},
-    isBST cmp h ->
-      forall x : A,
-        Elem x (bigger pivot h)
-          <->
-        Elem x h /\ x > pivot.
-Proof.
-  intros until h.
-  functional induction bigger pivot h;
-  isBST; intro;
-  rewrite ?Elem_node, ?IHs; auto;
-  split; Elems'.
-Qed.
-
-Lemma isBST_bigger :
-  forall (A : Ord) (pivot : A) (h : SplayTree A),
-    isBST cmp h -> isBST cmp (bigger pivot h).
-Proof.
-  intros until h.
-  functional induction bigger pivot h;
-  isBST'; auto; intros.
-    apply Elem_bigger in H; firstorder.
-    apply Elem_bigger in H; firstorder.
-    inv H.
-      trich.
-      specialize (H6 _ H1). specialize (H4 v' ltac:(auto)). trich.
-Qed.
-
-Lemma bigger_elem' :
-  forall (A : Ord) (x pivot : A) (h : SplayTree A),
-    isBST cmp h -> elem cmp x h -> pivot ≤ x -> pivot <> x ->
-      elem cmp x (bigger pivot h).
-Proof.
-  intros until h. revert x.
-  functional induction bigger pivot h;
-  intro; isBST.
-    Elem.
-    Elems. apply IHs; auto. trich.
-    Elem. trich. apply IHs; auto. trich.
-    Elem. trich; apply IHs; trich.
-      specialize (H4 v' ltac:(auto)). trich.
-      specialize (H4 v' ltac:(auto)). trich.
-Qed.
-
-(** Properties of [smaller]. *)
-
-Lemma smaller_spec :
-  forall {A : Ord} {pivot : A} {h : SplayTree A},
-    isBST cmp h -> forall x : A, elem cmp x (smaller pivot h) -> x ≤ pivot.
-Proof.
-  intros until h.
-  functional induction smaller pivot h;
-  isBST; inv 1.
-    trich.
-    trich. specialize (IHs H8 _ H1). trich.
-    trich. specialize (IHs H2 _ H1). trich.
-Qed.
-
-Lemma Elem_smaller : (* TODO: fix definition of isBST *)
-  forall {A : Ord} {pivot : A} {h : SplayTree A},
-    isBST cmp h ->
-      forall x : A,
-        Elem x (smaller pivot h)
-          <->
-        Elem x h /\ x < pivot.
-Proof.
-  intros until h.
-  functional induction smaller pivot h;
-  isBST; intro;
-  rewrite ?Elem_node, ?IHs; auto;
-  split; Elems'.
-Admitted.
-
-Lemma isBST_smaller :
-  forall {A : Ord} {pivot : A} {h : SplayTree A},
-    isBST cmp h -> isBST cmp (smaller pivot h).
-Proof.
-  intros until h.
-  functional induction smaller pivot h;
-  isBST'; try intro;
-  rewrite ?Elem_smaller; Elems'.
-    specialize (H6 v' ltac:(auto)). trich.
-    specialize (H6 v' ltac:(auto)). trich.
-Qed.
-
-(** Properties of [partition]. *)
-
-Lemma Elem_partition :
-  forall {A : Ord} {pivot : A} {h l r : SplayTree A},
-    partition pivot h = (l, r) ->
-      isBST cmp h ->
-        forall x : A, Elem x h <-> Elem x l \/ Elem x r.
-Proof.
-  unfold partition.
-  inv 1. intros.
-  rewrite Elem_smaller, Elem_bigger.
-    2-3: assumption.
-    firstorder. destruct (cmp_spec x pivot).
-      admit. (* TODO: fix definition of isBST *)
-      left. split; try left; auto.
-      right; split; auto.
-Admitted.
-
-Lemma isBST_partition :
-  forall {A : Ord} {pivot : A} {h l r : SplayTree A},
-    partition pivot h = (l, r) ->
-      isBST cmp h -> isBST cmp (node pivot l r).
-Proof.
-  unfold partition.
-  inv 1. isBST'.
-    apply isBST_smaller. assumption.
-    intro. rewrite Elem_smaller; Elems'.
-    apply isBST_bigger. assumption.
-    intro. rewrite Elem_bigger; Elems'.
-Qed.
-
-Lemma size_partition :
-  forall {A : Ord} {pivot : A} {h l r : SplayTree A},
-    partition pivot h = (l, r) ->
-      isBST cmp h -> size h = size l + size r.
-Proof.
-  unfold partition. inv 1.
-  functional induction smaller pivot h;
-  isBST; cbn; trich.
-    rewrite IHs; auto; lia.
-    functional induction bigger pivot l';
-    cbn.
-      lia.
-      cbn in *.
-Abort.
-
-(** Properties of [insert]. *)
-
-Lemma Elem_insert :
-  forall {A : Ord} {x : A} {h : SplayTree A},
-    isBST cmp h ->
-      forall y : A, Elem y (insert x h) <-> y = x \/ Elem y h.
-Proof.
-  unfold insert, partition. intros.
-  rewrite Elem_node, Elem_smaller, Elem_bigger; auto. split.
-    firstorder.
-    destruct (cmp_spec y x); firstorder.
-Qed.
-
-Lemma isBST_insert :
-  forall {A : Ord} {x : A} {h : SplayTree A},
-    isBST cmp h -> isBST cmp (insert x h).
-Proof.
-  intros.
-  unfold insert.
-  destruct (partition x h) eqn: Heq.
-  eapply isBST_partition; eassumption.
-Qed.
-
-(** Properties of [merge]. *)
-
-Lemma Elem_merge :
-  forall {A : Ord} {h1 h2 : SplayTree A} {x : A},
-    isBST cmp h1 -> isBST cmp h2 ->
-      Elem x (merge h1 h2)
-        <->
-      Elem x h1 \/ Elem x h2.
-Proof.
-  intros until h2.
-  functional induction merge h1 h2;
-  intro; isBST.
-    split; Elems.
-    {
-      pose (isBST_partition e0 H). inv i.
-      rewrite (Elem_partition e0 H), ?Elem_node, IHs, IHs0; auto.
-      split; Elems''.
-    }
-Qed.
-
-Lemma isBST_merge :
-  forall {A : Ord} {h1 h2 : SplayTree A},
-    isBST cmp h1 -> isBST cmp h2 ->
-      isBST cmp (merge h1 h2).
-Proof.
-  intros until h2.
-  functional induction merge h1 h2;
-  isBST.
-    assumption.
-    pose (isBST_partition e0 H). isBST'.
-      apply IHs; assumption.
-      intro. rewrite Elem_merge; Elems.
-      apply IHs0; assumption.
-      intro. rewrite Elem_merge; Elems.
 Qed.
