Sorting/SplaySort.v
@@ -8,27 +8,6 @@ Require Export SplayTree.
 
 Set Implicit Arguments.
 
-Lemma size_deleteMin :
-  forall (A : Ord) (h : SplayTree A),
-    size (deleteMin h) = pred (size h).
-Proof.
-  intros. functional induction deleteMin h; cbn; try reflexivity.
-  rewrite IHs. destruct l; cbn.
-    contradiction.
-    reflexivity.
-Qed.
-
-Lemma size_deleteMin' :
-  forall (A : Ord) (t t' : SplayTree A),
-    t' = snd (deleteMin' t) -> size t' = pred (size t).
-Proof.
-  intros. revert t' H.
-  functional induction deleteMin' t; inv 1; cbn in *.
-  destruct l; cbn.
-    contradiction.
-    rewrite e0 in IHp. cbn in IHp. rewrite IHp; reflexivity.
-Qed.
-
 Fixpoint fromList {A : Type} (p : A -> A -> bool) (l : list A) : SplayTree A :=
 match l with
     | [] => empty
@@ -36,7 +15,7 @@ match l with
 end.
 
 Definition splaySort {A : Type} (p : A -> A -> bool) (l : list A) : list A :=
-  BTree_toList (fromList p l).
+  inorder (fromList p l).
 
 Lemma isBST_fromList :
   forall (A : Type) (p : A -> A -> comparison) (l : list A),
@@ -51,34 +30,16 @@ Theorem Sorted_splaySort :
   forall {A : Ord} (l : list A),
     Sorted cmp (splaySort cmp l).
 Proof.
-  intros. unfold splaySort. apply Sorted_BTree_toList, isBST_fromList.
+  intros. unfold splaySort. apply Sorted_inorder, isBST_fromList.
 Qed.
 
-Lemma countBT_fromList :
-  forall (A : Type) (cmp : A -> A -> bool) (p : A -> bool) (l : list A),
-    countBT p (fromList cmp l) = Perm.count p l.
-Proof.
-  induction l as [| h t]; cbn.
-    reflexivity.
-    rewrite countBT_insert. rewrite IHt.
-      destruct (p h); reflexivity.
-Qed.
-
-Theorem splaySort_perm :
-  forall (A : Type) (cmp : A -> A -> bool) (l : list A),
-    perm l (splaySort cmp l).
-Proof.
-  unfold splaySort, perm. intros.
-  rewrite count_toList. rewrite countBT_fromList. reflexivity.
-Qed.
-
-Lemma Permutation_partition :
+Lemma Permutation_splay :
   forall (A : Ord) (p : A -> A -> bool) (pivot : A) (h h1 h2 : SplayTree A),
-    partition p pivot h = (h1, h2) ->
-      Permutation (BTree_toList h) (BTree_toList h1 ++ BTree_toList h2).
+    splay p pivot h = (h1, h2) ->
+      Permutation (inorder h) (inorder h1 ++ inorder h2).
 Proof.
   intros A p pivot h.
-  functional induction @partition A p pivot h; cbn in *; inv 1.
+  functional induction @splay A p pivot h; cbn in *; inv 1.
     cbn. rewrite app_nil_r. reflexivity.
     cbn. rewrite <- !app_assoc. cbn. apply Permutation_app.
       reflexivity.
@@ -93,24 +54,84 @@ Proof.
     rewrite (IHp0 _ _ e3). cbn. rewrite <- !app_assoc. reflexivity.
 Qed.
 
-Lemma Permutation_BTree_toList_insert :
+Lemma Permutation_inorder_insert :
   forall (A : Ord) (p : A -> A -> bool) (x : A) (t : BTree A),
-    Permutation (BTree_toList (insert p x t)) (x :: BTree_toList t).
+    Permutation (inorder (insert p x t)) (x :: inorder t).
 Proof.
   induction t as [| v l r]; cbn.
     reflexivity.
-    unfold insert. destruct (partition p x (node v l t1)) eqn: Heq.
+    unfold insert. destruct (splay p x (node v l t1)) eqn: Heq.
       cbn. rewrite Permutation_app_comm. cbn. constructor.
-        rewrite (@Permutation_partition _ _ _ _ _ _ Heq).
+        rewrite (@Permutation_splay _ _ _ _ _ _ Heq).
           apply Permutation_app_comm.
 Qed.
 
-Lemma Permutation_splaySort :
+Theorem Permutation_splaySort :
   forall (A : Ord) (p : A -> A -> bool) (l : list A),
     Permutation (splaySort p l) l.
 Proof.
   intros. unfold splaySort.
   induction l as [| h t]; cbn.
     reflexivity.
-    rewrite Permutation_BTree_toList_insert. constructor. assumption.
+    rewrite Permutation_inorder_insert. constructor. assumption.
+Qed.
+
+Instance Sort_splaySort (A : Ord) : Sort cmp :=
+{
+    sort := splaySort trich_leb;
+    Sorted_sort := Sorted_splaySort;
+    Permutation_sort := Permutation_splaySort A cmp;
+}.
+
+(* Another way to prove permutation properties *)
+
+Lemma countBT_splay :
+  forall (A : Type) (cmp : A -> A -> bool) (p : A -> bool) (pivot : A) (h h1 h2 : SplayTree A),
+    splay cmp pivot h = (h1, h2) ->
+      countBT p h = countBT p h1 + countBT p h2.
+Proof.
+  intros until h. revert p.
+  functional induction splay cmp pivot h;
+  inv 1; cbn; erewrite IHp; eauto;
+  destruct (p x), (p y); cbn; unfold id; lia.
+Qed.
+
+Lemma countBT_insert :
+  forall (A : Type) (cmp : A -> A -> bool) (p : A -> bool) (x : A) (h : SplayTree A),
+    countBT p (insert cmp x h) =
+    (if p x then 1 else 0) + countBT p h.
+Proof.
+  intros. unfold insert.
+  destruct (splay cmp x h) eqn: Heq.
+  apply (countBT_splay cmp p) in Heq.
+  rewrite Heq. cbn. destruct (p x); reflexivity.
+Qed.
+
+Lemma countBT_merge :
+  forall (A : Type) (cmp : A -> A -> bool) (p : A -> bool) (h1 h2 : SplayTree A),
+    countBT p (merge cmp h1 h2) = countBT p h1 + countBT p h2.
+Proof.
+  intros until h2.
+  functional induction (merge cmp h1 h2); cbn.
+    reflexivity.
+    apply (countBT_splay cmp p) in e0.
+      destruct (p v); unfold id; lia.
+Qed.
+
+Lemma countBT_fromList :
+  forall (A : Type) (cmp : A -> A -> bool) (p : A -> bool) (l : list A),
+    countBT p (fromList cmp l) = Perm.count p l.
+Proof.
+  induction l as [| h t]; cbn.
+    reflexivity.
+    rewrite countBT_insert. rewrite IHt.
+      destruct (p h); reflexivity.
+Qed.
+
+Theorem perm_splaySort :
+  forall (A : Type) (cmp : A -> A -> bool) (l : list A),
+    perm l (splaySort cmp l).
+Proof.
+  unfold splaySort, perm. intros.
+  rewrite count_toList. rewrite countBT_fromList. reflexivity.
 Qed.
